checkpoint further progress on lithium tutorial

new/golang/theory/lithium/lithium.v
@@ -11,6 +11,8 @@ From lithium Require Import hooks all.
 
 Set Default Proof Using "Type".
 
+(* copy of lithium tutorial, applied to GooseLang *)
+
 (** * Definitions of Lithium functions *)
 (** First, we define the Lithium functions that we will use later. *)
 Section definitions.
@@ -25,7 +27,7 @@ Section definitions.
   Definition unop_ok (op : un_op) (v : val) (G : val → iProp Σ) : iProp Σ :=
     WP UnOp op v {{ G }}.
 
-  Definition if_ok (v : val) (G1 G2 : iProp Σ) : iProp Σ :=
+  Definition if_ok `{!goGlobalsGS Σ} (v : val) (G1 G2 : iProp Σ) : iProp Σ :=
     ∃ b : bool, ⌜v = #b⌝ ∗ if b then G1 else G2.
 End definitions.
 
@@ -42,7 +44,7 @@ Section setup.
   Class UnopOk (op : un_op) (v : val) : Type :=
     unop_ok_proof G : iProp_to_Prop (unop_ok op v G).
   Class IfOk (v : val) : Type :=
-    if_ok_proof G1 G2 : iProp_to_Prop (Σ:=Σ) (if_ok v G1 G2).
+    if_ok_proof G1 G2 : iProp_to_Prop (if_ok v G1 G2).
 End setup.
 
 Ltac generate_i2p_instance_to_tc_hook arg c ::=
@@ -184,4 +186,708 @@ Section proofs.
     iStartProof. unfold assert_two.
     repeat liTStep; liShow.
   Qed.
+
+  (** ** 2. Operational model *)
+  (** The operational semantics of Lithium are given by the [liTStep]
+  tactic that executes one step of the Lithium interpreter. The state
+  of the Lithium interpreter is of the form:
+
+                           Γ; Δ |- ∃ x, G(x)
+
+  where Γ is the Coq context, Δ is the Iris context, x is a tuple of
+  existential quantifiers and G is the current Lithium program. Each
+  step of the Lithium interpreter (i.e., each [liTStep]) transforms
+  the state into a new state, i.e. it can be described mathematically
+  as a transition
+
+       Γ1; Δ1 |- ∃ x1, G1(x1) => Γ2; Δ2 |- ∃ x2, G2(x2)
+
+  The execution ends when Lithium reaches [done]. A mathematical
+  description of the steps of the Lithium interpreter can be found in
+  Michael Sammler's dissertation. *)
+
+  (** ** 3. Modular verification via inhale, exhale and quantifiers *)
+  Definition add1 : val := λ: "v", "v" + #(W64 1).
+
+  Definition fn_ok (v : val) (X : Type)
+    (pre : X → val → iProp Σ) (post : X → val → iProp Σ) : iProp Σ :=
+    □ ∃ f b e, ⌜v = RecV f b e⌝ ∗
+    ∀ x va, pre x va -∗ ▷ WP subst' b va (subst' f v e) {{ vr, post x vr}}.
+  Global Typeclasses Opaque fn_ok.
+
+  Global Instance fn_ok_pers X v pre post :
+    Persistent (fn_ok v X pre post).
+  Proof. unfold fn_ok. apply _. Qed.
+
+  Global Instance fn_ok_intro_pers X v pre post :
+    IntroPersistent (fn_ok v X pre post) (fn_ok v X pre post).
+  Proof. constructor. by iIntros "#?". Qed.
+
+  Lemma prove_fn_ok X f a e pre post :
+    fn_ok (RecV f a e) X pre post :-
+      drop_spatial;
+      ∀ (x : X) v vr,
+      inhale pre x v;
+      inhale fn_ok vr X pre post;
+      v' ← {expr_ok (subst' a v (subst' f vr e))};
+      exhale post x v';
+      done.
+  Proof.
+    liTUnfold. unfold fn_ok. iIntros "#HWP !>".
+    iExists _, _, _. iSplit; [done|].
+    iIntros (x va) "Hpre". iModIntro.
+    iLöb as "IH" forall (x va).
+    iApply (wp_wand with "[-]").
+    - iApply ("HWP" with "Hpre").
+      iModIntro. iExists _, _, _. iSplit; [done|].
+      iIntros (??) "?". iModIntro. by iApply "IH".
+    - iIntros (?) "[$ _]".
+  Qed.
+
+  Lemma add1_correct :
+    ⊢ fn_ok add1 w64
+        (λ (n: w64) (v: val), ⌜v = #n⌝)
+        (λ (n: w64) (v: val), ⌜v = #(word.add n (W64 1))⌝).
+  Proof.
+    iStartProof. iApply prove_fn_ok. simpl.
+    repeat liTStep; liShow.
+  Qed.
+
+  Definition assert_two_modular (add1 : val) : expr :=
+    let: "x" := #(W64 1) in
+    let: "y" := add1 "x" in
+    std.Assert ("y" = #(W64 2)).
+
+  (** These find functions are explained in 5. *)
+  Definition FindFnOk (v : val) :=
+  {| fic_A := sigT (λ X, (X → val → iProp Σ) * (X → val → iProp Σ))%type;
+    fic_Prop '(existT X (pre, post)) := fn_ok v X pre post |}.
+  Global Typeclasses Opaque FindFnOk.
+  Lemma find_in_context_find_fn_ok v G:
+    find_in_context (FindFnOk v) G :-
+      pattern: X pre post, fn_ok v X pre post; return G (existT X (pre, post)).
+  Proof. iDestruct 1 as (X pre post) "[Hv HT]". iExists _. by iFrame. Qed.
+  Definition find_in_context_find_fn_ok_inst :=
+    [instance find_in_context_find_fn_ok with FICSyntactic].
+  Global Existing Instance find_in_context_find_fn_ok_inst | 1.
+
+  Lemma expr_app e1 e2 G :
+    expr_ok (App e1 e2) G  :-
+      v2 ← {expr_ok e2};
+      v1 ← {expr_ok e1};
+      '(existT X (pre, post)) ← find_in_context (FindFnOk v1);
+      ∃ x,
+      exhale (pre x v2);
+      ∀ v',
+      inhale (post x v');
+      return G v'.
+  Proof.
+    liTUnfold. iIntros "HWP". wp_bind (e2). iApply (wp_wand with "HWP").
+    iIntros (?) "HWP". wp_bind (e1). iApply (wp_wand with "HWP").
+    iIntros (?) "[%a HWP]". destruct a as [?[??]] => /=. unfold fn_ok.
+    iDestruct "HWP" as "[#(%&%&%&->&Hf) [% [Hpre HG]]]".
+    iDestruct ("Hf" with "[$]") as "HWP".
+    wp_pures. by iApply (wp_wand with "HWP").
+  Qed.
+  Definition expr_app_inst := [instance expr_app].
+  Global Existing Instance expr_app_inst | 50.
+
+
+  Lemma assert_two_modular_correct add1 :
+    ⊢ [{
+      inhale fn_ok add1 w64 (λ n v, ⌜v = #n⌝) (λ n v, ⌜v = #(word.add n 1)⌝);
+      _ ← {expr_ok (assert_two_modular add1)};
+      done
+    } ].
+  Proof.
+    iStartProof. unfold assert_two_modular.
+    repeat liTStep; liShow.
+  Qed.
+
+  (** ** 4. Continuations *)
+  Definition fib : val := rec: "f" "x" :=
+      if: "x" = #(W64 0) then
+        #(W64 0)
+      else if: "x" = #(W64 1) then
+        #(W64 1)
+      else
+         "f" ("x" - #(W64 1)) + "f" ("x" - #(W64 2)).
+
+  Lemma expr_if e0 e1 e2 G :
+    expr_ok (If e0 e1 e2) G :-
+      v ← {expr_ok e0};
+      {if_ok v (expr_ok e1 G) (expr_ok e2 G)}.
+  Proof.
+    liTUnfold. iIntros "HWP". wp_bind (e0).
+    iApply (wp_wand with "HWP"). iIntros (?) "[%b [-> HWP]]".
+    by destruct b; wp_pures.
+  Qed.
+  Definition expr_if_inst := [instance expr_if].
+  Global Existing Instance expr_if_inst.
+
+  Lemma if_bool (b : bool) (G1 G2: iProp Σ) :
+    if_ok #b G1 G2 :-
+      if: b
+      | return G1
+      | return G2.
+  Proof.
+    liTUnfold. iIntros "Hif".
+    iExists _. iSplit; [done|].
+    destruct b.
+    - iDestruct "Hif" as "[HG _]". by iApply "HG".
+    - iDestruct "Hif" as "[_ HG]". iApply "HG". naive_solver.
+  Qed.
+  Definition if_bool_inst := [instance if_bool].
+  Global Existing Instance if_bool_inst | 10.
+
+  (*
+  Lemma fib_correct :
+    ⊢ fn_ok fib unit (λ _ v, ∃ n : w64, ⌜v = #n⌝ ∗ ⌜(0 ≤ uint.Z n)%Z⌝)
+        (λ _ v, ∃ n' : w64, ⌜v = #n'⌝ ∗ ⌜(0 ≤ uint.Z n')%Z⌝).
+  Proof.
+    iStartProof. iApply prove_fn_ok. simpl.
+    liTStep.
+    liTStep.
+    liTStep.
+    liTStep.
+    liTStep.
+    liTStep.
+    liTStep.
+    liTStep.
+    liTStep.
+    liTStep.
+    liTStep.
+    liTStep.
+    liTStep.
+    liTStep.
+    liTStep.
+    liTStep.
+    liTStep.
+    liTStep.
+    liTStep.
+    1: repeat liTStep.
+
+    do 8 liTStep.
+    1: {
+      liTStep; liShow.
+
+      iClear "#".
+
+      liTStep; liShow.
+      liTStep; liShow.
+      liTStep; liShow.
+      liTStep; liShow.
+      liTStep; liShow.
+      liTStep; liShow.
+    }
+
+    do 10 liTStep.
+    liTStep; liShow.
+    liTStep; liShow.
+
+
+    repeat liTStep; liShow.
+    iExists (li_pair _ _).
+    repeat liTStep; liShow.
+    iExists _.
+    repeat liTStep; liShow.
+    iExists _.
+    repeat liTStep; liShow.
+    Unshelve. all: unshelve_sidecond.
+    - lia.
+    - lia.
+    - lia.
+  Qed.
+*)
+
+  (** ** 5. Separation logic *)
+  Lemma expr_alloc `{!IntoVal V} (v: V) G :
+    expr_ok (mem.alloc #v) G :-
+      ∀ (l: loc),
+      inhale (l ↦ v);
+      return G #l.
+  Proof. liTUnfold. iIntros "HG". by iApply wp_alloc. Qed.
+  Definition expr_alloc_inst := [instance @expr_alloc].
+  Global Existing Instance expr_alloc_inst.
+
+  Definition FindPointsTo (l : loc) :=
+  {| fic_A := sigT (fun (V: Type) => (IntoVal V * V)%type);
+     fic_Prop '(existT V (_, v)) := (l ↦ v)%I; |}.
+  Global Typeclasses Opaque FindPointsTo.
+
+  (* Questions:
+
+  Why are these lemmas for Store e1 e2 (arbitrary expressions) and not values?
+  Can we make them values and add wp_pures automation in between?
+
+  How do we deal with the fact that functions take only argument?
+
+  *)
+
+  Lemma expr_store e1 e2 G :
+    expr_ok (Store e1 e2) G :-
+      v2 ← {expr_ok e2};
+      ∀ (V2: Type) (H: IntoVal V2) (v2': V2),
+      exhale ⌜v2 = #v2'⌝;
+      v1 ← {expr_ok e1};
+      ∀ (l1: loc),
+      exhale ⌜v1 = #l1⌝;
+      (* TODO: we can actually do a FindPointsTo with a fixed value type of V2 *)
+      _ ← find_in_context (FindPointsTo l1);
+      inhale (l1 ↦ v2');
+      return G v2.
+  Proof.
+    (*
+    liTUnfold. iIntros "HWP". wp_bind (e2).
+    iApply (wp_wand with "HWP"). iIntros (?) "HWP".
+    wp_bind (e1). iApply (wp_wand with "HWP"). iIntros (?) "[% [? HWP]]/=".
+    by iApply (wp_store with "[$]").
+    *)
+  Abort.
+
+  (* rest of tutorial *)
+
+  (*
+  Definition expr_store_inst := [instance expr_store].
+  Global Existing Instance expr_store_inst.
+
+  Lemma expr_load e G :
+    expr_ok (Load e) G :-
+      v ← {expr_ok e};
+      vl ← find_in_context (FindPointsTo v);
+      inhale (v ↦ vl);
+      return G vl.
+  Proof.
+    liTUnfold. iIntros "HWP". wp_bind (e).
+    iApply (wp_wand with "HWP"). iIntros (?) "[% [? HWP]]/=".
+    by iApply (wp_load with "[$]").
+  Qed.
+  Definition expr_load_inst := [instance expr_load].
+  Global Existing Instance expr_load_inst.
+
+
+  Lemma find_points_to v1 G:
+    find_in_context (FindPointsTo v1) G :-
+      pattern: v, v1 ↦ v; return G v.
+  Proof. iDestruct 1 as (v) "[Hl HT]". iExists _ => /=. by iFrame. Qed.
+  Definition find_points_to_inst :=
+    [instance find_points_to with FICSyntactic].
+  Global Existing Instance find_points_to_inst | 1.
+
+  Global Instance related_to_points_to A vl v : RelatedTo (λ x : A, vl ↦ v x)%I | 100 :=
+    {| rt_fic := FindPointsTo vl |}.
+
+  Lemma expr_load_alt e G :
+    expr_ok (Load e) G :-
+      v ← {expr_ok e};
+      ∃ vl, exhale (v ↦ vl);
+      inhale (v ↦ vl);
+      return G vl.
+  Proof.
+    liTUnfold. iIntros "HWP". wp_bind (e).
+    iApply (wp_wand with "HWP"). iIntros (?) "[% [? HWP]]/=".
+    by iApply (wp_load with "[$]").
+  Qed.
+  Definition expr_load_alt_inst := [instance expr_load_alt].
+
+  Lemma subsume_points_to_points_to A vl v1 v2 G :
+    subsume (vl ↦ v1) (λ x : A, vl ↦ (v2 x)) G :-
+     ∃ x, exhale ⌜v1 = v2 x⌝;
+     return G x.
+  Proof. liTUnfold. iIntros "[% [-> ?]] ?". iExists _. iFrame. Qed.
+  Definition subsume_points_to_points_to_inst := [instance subsume_points_to_points_to].
+  Global Existing Instance subsume_points_to_points_to_inst.
+
+  Definition points_to_test : val := λ: <>,
+      let: "l" := Alloc in
+      "l" <- !"l";;
+      "l".
+
+  Lemma points_to_test_correct :
+    ⊢ fn_ok points_to_test unit (λ _ _, True) (λ _ v, ∃ z : Z, v ↦ #z ∗ ⌜0 ≤ z⌝).
+  Proof.
+    iStartProof. iApply prove_fn_ok. simpl.
+    repeat liTStep; liShow.
+  Qed.
+
+  Section alt.
+    Local Existing Instance expr_load_alt_inst | 0.
+    Lemma points_to_test_correct_alt :
+      ⊢ fn_ok points_to_test unit (λ _ _, True) (λ _ v, ∃ z : Z, v ↦ #z ∗ ⌜0 ≤ z⌝).
+    Proof.
+      iStartProof. iApply prove_fn_ok. simpl.
+      repeat liTStep; liShow.
+    Qed.
+  End alt.
+
+  (** ** 6. Reasoning about abstract predicates  *)
+
+  Fixpoint is_list (v : val) (xs : list val) : iProp Σ :=
+    match xs with
+    | [] => ⌜v = #NULL⌝
+    | x :: xs => ∃ vnext, v ↦ (x, vnext)%V ∗ is_list vnext xs
+  end.
+  Global Typeclasses Opaque is_list.
+  Global Opaque is_list.
+
+  Lemma is_list_cons v x xs :
+    is_list v (x::xs) = (∃ vnext, v ↦ (x, vnext)%V ∗ is_list vnext xs)%I.
+  Proof. done. Qed.
+  Lemma is_list_NULL v xs :
+    is_list v xs -∗ ⌜xs = [] ↔ v = #NULL⌝.
+  Proof.
+    destruct xs. { unfold_opaque is_list. naive_solver. }
+    rewrite is_list_cons. iDestruct 1 as (?) "[Hv _]".
+    unfold val_pointsto. iDestruct "Hv" as (? ->) "?". naive_solver.
+  Qed.
+
+  (** *** Lithium rules for pairs *)
+  (** These rules are used by the functions on lists. *)
+  Lemma expr_unop op e G :
+    expr_ok (UnOp op e) G :-
+      v  ← {expr_ok e};
+      vr ← {unop_ok op v};
+      return G vr.
+  Proof.
+    liTUnfold. iIntros "HWP". wp_bind (e).
+    iApply (wp_wand with "HWP"). by iIntros (?) "HWP".
+  Qed.
+  Definition expr_unop_inst := [instance expr_unop].
+  Global Existing Instance expr_unop_inst.
+
+  Lemma unop_fst v1 v2 G :
+    unop_ok FstOp (v1, v2) G :- return G v1.
+  Proof. liTUnfold. iIntros "HG". by wp_pures. Qed.
+  Definition unop_fst_inst := [instance unop_fst].
+  Global Existing Instance unop_fst_inst.
+  Lemma unop_snd v1 v2 G :
+    unop_ok SndOp (v1, v2) G :- return G v2.
+  Proof. liTUnfold. iIntros "HG". by wp_pures. Qed.
+  Definition unop_snd_inst := [instance unop_snd].
+  Global Existing Instance unop_snd_inst.
+
+  Lemma binop_pair v1 v2 G :
+    binop_ok PairOp v1 v2 G :- return G (v1, v2)%V.
+  Proof. liTUnfold. iIntros "HG". by wp_pures. Qed.
+  Definition binop_pair_inst := [instance binop_pair].
+  Global Existing Instance binop_pair_inst.
+
+  (** *** Constructing linked lists *)
+  Definition empty_code : val := λ: <>, #NULL.
+  Definition cons_code : val := λ: "a",
+      let: "v" := Fst "a" in
+      let: "l" := Snd "a" in
+      let: "new_l" := Alloc in
+      "new_l" <- ("v", "l");;
+      "new_l".
+
+  Definition mklist_code (empty cons : val) : val := λ: <>,
+    let: "l" := empty #0 in
+    let: "l" := cons (#1, "l") in
+    let: "l" := cons (#2, "l") in
+    "l".
+
+
+  Lemma empty_code_correct :
+    ⊢ fn_ok empty_code unit (λ _ _, True) (λ _ v, is_list v []).
+  Proof.
+    iStartProof. iApply prove_fn_ok. simpl.
+    repeat liTStep; liShow.
+  Abort.
+
+  Lemma simpl_list_empty xs G :
+    simplify_goal (is_list #NULL xs) G :- exhale ⌜xs = []⌝; return G.
+  Proof. liTUnfold. iIntros "[-> $]". by unfold_opaque is_list. Qed.
+  Definition simpl_list_empty_inst := [instance simpl_list_empty with 50%N].
+  Global Existing Instance simpl_list_empty_inst.
+
+  Lemma empty_code_correct :
+    ⊢ fn_ok empty_code unit (λ _ _, True) (λ _ v, is_list v []).
+  Proof.
+    iStartProof. iApply prove_fn_ok. simpl.
+    repeat liTStep; liShow.
+  Qed.
+
+
+  Lemma cons_correct :
+    ⊢ fn_ok cons_code (val * list val)
+      (λ '(x, xs) a, ∃ v, ⌜a = (x, v)%V⌝ ∗ is_list v xs)
+      (λ '(x, xs) r, is_list r (x :: xs)).
+  Proof.
+    iStartProof. iApply prove_fn_ok. simpl.
+    repeat liTStep; liShow.
+  Abort.
+
+  Definition FindList (v : val) :=
+  {| fic_A := iProp Σ; fic_Prop P := P; |}.
+  Global Typeclasses Opaque FindList.
+  Global Instance related_to_list A v xs : RelatedTo (λ x : A, is_list v (xs x)) | 100
+    := {| rt_fic := FindList v |}.
+
+  Lemma find_list v G:
+    find_in_context (FindList v) G :-
+      pattern: xs, is_list v xs; return G (is_list v xs).
+  Proof. iDestruct 1 as (xs) "[Hl HT]". iExists _. by iFrame. Qed.
+  Definition find_list_inst :=
+    [instance find_list with FICSyntactic].
+  Global Existing Instance find_list_inst | 1.
+
+  Lemma find_list_points_to v G:
+    find_in_context (FindList v) G :-
+      pattern: v2, v ↦ v2; return G (v ↦ v2).
+  Proof. iDestruct 1 as (?) "[Hl HT]". iExists _. by iFrame. Qed.
+  Definition find_list_points_to_inst :=
+    [instance find_list_points_to with FICSyntactic].
+  Global Existing Instance find_list_points_to_inst | 10.
+
+  Lemma subsume_list_list A v xs1 xs2 G :
+    subsume (is_list v xs1) (λ x : A, is_list v (xs2 x)) G :-
+     ∃ x, exhale ⌜xs1 = xs2 x⌝;
+     return G x.
+  Proof. liTUnfold. iIntros "[% [-> ?]] ?". iExists _. iFrame. Qed.
+  Definition subsume_list_list_inst := [instance subsume_list_list].
+  Global Existing Instance subsume_list_list_inst.
+
+  Lemma subsume_points_to_list A vl v xs G :
+    subsume (vl ↦ v) (λ x : A, is_list vl (xs x)) G :-
+     ∃ x v1 v2 xs',
+     exhale ⌜v = (v1, v2)%V⌝ ∗ is_list v2 xs' ∗ ⌜xs x = v1 :: xs'⌝;
+     return G x.
+  Proof.
+    liTUnfold. iIntros "[% [% [% [% [[-> [Hl %Hxs]] ?]]]]] ?".
+    iExists _. iFrame. rewrite Hxs is_list_cons. iExists _. iFrame.
+  Qed.
+  Definition subsume_points_to_list_inst := [instance subsume_points_to_list].
+  Global Existing Instance subsume_points_to_list_inst.
+
+
+  Lemma cons_correct :
+    ⊢ fn_ok cons_code (val * list val)
+      (λ '(x, xs) a, ∃ v, ⌜a = (x, v)%V⌝ ∗ is_list v xs)
+      (λ '(x, xs) r, is_list r (x :: xs)).
+  Proof.
+    iStartProof. iApply prove_fn_ok. simpl.
+    repeat liTStep; liShow.
+  Qed.
+
+  Lemma mklist_correct empty cons :
+    fn_ok empty unit (λ _ _, True) (λ _ v, is_list v []) -∗
+    fn_ok cons (val * list val) (λ '(x, xs) a, ∃ v, ⌜a = (x, v)%V⌝ ∗ is_list v xs) (λ '(x, xs) r, is_list r (x :: xs)) -∗
+    fn_ok (mklist_code empty cons) unit (λ _ _, True) (λ _ v, is_list v [ #2; #1 ]).
+  Proof.
+    iStartProof. iIntros "#? #?". iApply prove_fn_ok. simpl.
+    repeat liTStep; liShow.
+  Qed.
+
+  (** *** Destructing linked lists *)
+  Definition head_code : val := λ: "l", Fst (! "l").
+
+  Lemma head_correct :
+    ⊢ fn_ok head_code (val * list val)
+      (λ '(va, xs) v, ⌜v = va⌝ ∗ is_list v xs ∗ ⌜0 < length xs⌝)
+      (λ '(va, xs) r, ⌜head xs = Some r⌝ ∗ is_list va xs).
+  Proof.
+    iStartProof. iApply prove_fn_ok. simpl.
+    repeat liTStep; liShow.
+  Abort.
+
+  Lemma find_points_to_list v G:
+    find_in_context (FindPointsTo v) G :-
+      pattern: xs, is_list v xs;
+      exhale ⌜0 < length xs⌝;
+      ∀ v' x xs',
+      inhale ⌜xs = x::xs'⌝ ∗ is_list v' xs';
+      return G (x, v')%V.
+  Proof.
+    liTUnfold. iIntros "[% [Hl [% HG]]]".
+    destruct xs => //=. rewrite is_list_cons.
+    iDestruct "Hl" as (?) "[??]". iExists _ => /=. iFrame.
+    iApply "HG". by iFrame.
+  Qed.
+  Definition find_points_to_list_inst :=
+    [instance find_points_to_list with FICSyntactic].
+  Global Existing Instance find_points_to_list_inst | 10.
+
+  Lemma head_correct :
+    ⊢ fn_ok head_code (val * list val)
+      (λ '(va, xs) v, ⌜v = va⌝ ∗ is_list v xs ∗ ⌜0 < length xs⌝)
+      (λ '(va, xs) r, ⌜head xs = Some r⌝ ∗ is_list va xs).
+  Proof.
+    iStartProof. iApply prove_fn_ok. simpl.
+    repeat liTStep; liShow.
+  Qed.
+
+  (** This tests that using [expr_load_alt] instead of [expr_load] works as well. *)
+  Section alt.
+    Local Existing Instance expr_load_alt_inst | 0.
+
+    Lemma head_correct_alt :
+      ⊢ fn_ok head_code (val * list val)
+        (λ '(va, xs) v, ⌜v = va⌝ ∗ is_list v xs ∗ ⌜0 < length xs⌝)
+        (λ '(va, xs) r, ⌜head xs = Some r⌝ ∗ is_list va xs).
+    Proof.
+      iStartProof. iApply prove_fn_ok. simpl.
+      repeat liTStep; liShow.
+    Qed.
+  End alt.
+
+  Definition length_code : val := rec: "f" "l" :=
+      if: "l" = #NULL then
+        #0
+      else
+        let: "r" := "f" (Snd (! "l")) in
+        "r" + #1.
+
+  Definition FindIsNULL (v : val) :=
+  {| fic_A := bool; fic_Prop b := (⌜b ↔ v = #NULL⌝ : iProp Σ)%I |}.
+  Global Typeclasses Opaque FindIsNULL.
+
+  Lemma binop_eq_NULL v G :
+    binop_ok EqOp v #NULL G :-
+      b ← find_in_context (FindIsNULL v);
+      return G #b.
+  Proof.
+    liTUnfold. iIntros "[% [Hb HG]]". simpl. iDestruct "Hb" as %?.
+    wp_pure _. 2: by iFrame.
+    simpl. repeat case_match; destruct b; naive_solver.
+  Qed.
+  Definition binop_eq_NULL_inst := [instance binop_eq_NULL].
+  Global Existing Instance binop_eq_NULL_inst.
+
+  Lemma find_null_points_to v G:
+    find_in_context (FindIsNULL v) G :-
+      pattern: v2, v ↦ v2;
+      inhale v ↦ v2;
+      return G false.
+  Proof.
+    liTUnfold.
+    iDestruct 1 as (?) "[Hl HG]".
+    unfold val_pointsto. iDestruct "Hl" as (? ->) "?".
+    iExists false => /=. iSplit; [naive_solver|]. iApply "HG".
+    iExists _. by iFrame.
+  Qed.
+  Definition find_null_points_to_inst :=
+    [instance find_null_points_to with FICSyntactic].
+  Global Existing Instance find_null_points_to_inst | 10.
+
+  Lemma find_null_list v G:
+    find_in_context (FindIsNULL v) G :-
+      pattern: xs, is_list v xs;
+      inhale is_list v xs;
+      return G (bool_decide (xs = [])).
+  Proof.
+    liTUnfold.
+    iDestruct 1 as (?) "[Hl HG]".
+    iDestruct (is_list_NULL with "Hl") as %?.
+    iExists _. iDestruct ("HG" with "Hl") as "$".
+    simpl. iPureIntro. naive_solver.
+  Qed.
+  Definition find_null_list_inst :=
+    [instance find_null_list with FICSyntactic].
+  Global Existing Instance find_null_list_inst | 10.
+
+  Lemma length_correct :
+    ⊢ fn_ok length_code (val * list val)
+      (λ '(va, xs) v, ⌜v = va⌝ ∗ is_list v xs)
+      (λ '(va, xs) r, ⌜r = #(length xs)⌝ ∗ is_list va xs).
+  Proof.
+    iStartProof. iApply prove_fn_ok. simpl.
+    repeat liTStep; liShow.
+    Unshelve. all: unshelve_sidecond.
+    - by destruct x0.
+    - do 2 f_equal. lia.
+  Qed.
+
+  (** ** 7. Verifying higher-order functions using Lithium *)
+
+  Definition contains_code : val := rec: "f" "x" :=
+      let: "l" := Fst "x" in
+      let: "cb" := Snd "x" in
+      if: "l" = #NULL then
+        #false
+      else if: "cb" (Fst (! "l")) then
+        #true
+      else
+        "f" (Snd (! "l"), "cb").
+
+  Global Instance related_to_fn_ok A v X pre post : RelatedTo (λ x : A, fn_ok v X (pre x) (post x)) | 100
+    := {| rt_fic := FindFnOk v |}.
+
+  Lemma subsume_fn A v X pre1 pre2 post1 post2 G :
+    subsume (fn_ok v X pre1 post1) (λ x : A, fn_ok v X pre2 post2) G :-
+     and:
+     | drop_spatial;
+       ∀ x v, inhale pre2 x v;
+       ∃ x', exhale pre1 x' v;
+       ∀ v', inhale post1 x' v';
+       exhale post2 x v';
+       done
+     | ∃ x, return G x.
+  Proof.
+    liTUnfold. iIntros "[#Hsub [% ?]] Hfn". iExists _. iFrame. unfold fn_ok.
+    iDestruct "Hfn" as "#[%[%[%[-> Hwp]]]]".
+    iModIntro. iExists _, _, _. iSplit; [done|].
+    iIntros (??) "?". iDestruct ("Hsub" with "[$]") as (?) "[Hpre1 HWP]".
+    iSpecialize ("Hwp" with "Hpre1"). iModIntro.
+    iApply (wp_wand with "Hwp"). iIntros (?) "Hpost1".
+    iDestruct ("HWP" with "Hpost1") as "[$ _]".
+  Qed.
+  Definition subsume_fn_inst := [instance subsume_fn].
+  Global Existing Instance subsume_fn_inst.
+
+  Lemma contains_correct (P : val → bool) :
+    ⊢ fn_ok contains_code (val * list val)
+      (λ '(va, xs) v, ∃ cb, ⌜v = (va, cb)%V⌝ ∗ is_list va xs ∗ fn_ok cb val (λ va v, ⌜v = va⌝ ∗ ⌜v ∈ xs⌝) (λ va v, ⌜v = #(P va)⌝))
+      (λ '(va, xs) r, ⌜r = #(bool_decide (Exists P xs))⌝ ∗ is_list va xs).
+  Proof.
+    iStartProof. iApply prove_fn_ok. simpl.
+    repeat liTStep; liShow.
+    Unshelve. all: unshelve_sidecond.
+    - by destruct x0.
+    - set_solver.
+    - do 2 f_equal. normalize_and_simpl_goal. constructor. naive_solver.
+    - set_solver.
+    - do 2 f_equal. apply bool_decide_ext. rewrite Exists_cons H0. naive_solver.
+  Qed.
+
+  Definition contains_one (contains : val) : val := λ: "x",
+      contains ("x", (λ: "y", "y" = #1)%V).
+
+  Lemma simpl_fn X f a e pre post G :
+    simplify_goal (fn_ok (RecV f a e) X pre post) G :-
+      and:
+      | drop_spatial;
+        ∀ (x : X) v vr,
+        inhale pre x v;
+        inhale fn_ok vr X pre post;
+        v' ← {expr_ok (subst' a v (subst' f vr e))};
+        exhale post x v';
+        done
+      | return G.
+  Proof. liTUnfold. iIntros "[Hsub $]". by iApply prove_fn_ok. Qed.
+  Definition simpl_fn_inst := [instance simpl_fn with 50%N].
+  Global Existing Instance simpl_fn_inst.
+
+  (* TODO: upstream? *)
+  Global Instance simpl_fmap_elem_of {A B} x (xs : list A) (f : A → B) :
+    SimplBoth (x ∈ f <$> xs) (∃ y, x = f y ∧ y ∈ xs).
+  Proof. constructor. by set_unfold. Qed.
+
+  Lemma contains_one_correct contains :
+    fn_ok contains (val * list val)
+      (λ '(va, xs) v, ∃ cb, ⌜v = (va, cb)%V⌝ ∗ is_list va xs ∗ fn_ok cb val (λ va v, ⌜v = va⌝ ∗ ⌜v ∈ xs⌝) (λ va v, ⌜v = #(bool_decide (va = #1))⌝))
+      (λ '(va, xs) r, ⌜r = #(bool_decide (Exists (λ x, (bool_decide (x = #1))) xs))⌝ ∗ is_list va xs)
+    -∗
+       fn_ok (contains_one contains) (val * list Z)
+      (λ '(va, xs) v, ⌜v = va⌝ ∗ is_list va (LitV <$> (LitInt <$> xs)))
+      (λ '(va, xs) r, ⌜r = #(bool_decide (1 ∈ xs))⌝ ∗ is_list va (LitV <$> (LitInt <$> xs))).
+  Proof.
+    iStartProof. iIntros "#?". iApply prove_fn_ok. simpl.
+    repeat liTStep; liShow.
+    Unshelve. all: unshelve_sidecond.
+    - repeat case_bool_decide; naive_solver.
+    - do 2 f_equal. apply bool_decide_ext. rewrite !Exists_fmap. rewrite Exists_exists. naive_solver.
+  Qed.
+  *)
+
 End proofs.
